\documentclass[11pt,a4paper]{article}
\usepackage[utf8]{inputenc}
\usepackage[english]{babel}
\usepackage{fontspec}
\usepackage{xunicode}
\usepackage{xltxtra}
\usepackage{polyglossia}
\usepackage{amsmath}
\usepackage{amsfonts}
\usepackage{amssymb}
\usepackage{graphicx}
\usepackage[left=2cm,right=2cm,top=2cm,bottom=2cm]{geometry}
\usepackage{afterpage}
\usepackage{xcolor}
\usepackage{pagecolor}
\usepackage{mathtools}
%\usepackage{fancyhdr}
\usepackage{hyperref}
\usepackage{blindtext}
\usepackage{mahjong}
\usepackage{amsthm}
\usepackage{chngcntr}
\usepackage{tikz}

\usepackage{stmaryrd}
\let\stmaryrdLightning\lightning

\author{Zehao Gao}

\begin{document}

\section*{Homework 3 solutions}

\paragraph*{Question 3}

\begin{enumerate}
\item[(a)]

\begin{equation}
    \vec{x}=
    \begin{pmatrix}
    x_1 \\
    x_2 \\
    x_3
    \end{pmatrix},\ 
    \vec{p}=
    \begin{pmatrix}
    p_1 \\
    p_2 \\
    p_3
    \end{pmatrix}
\end{equation}

\begin{equation}
    \hat{\vec{L}}=\hat{\vec{x}}\times\hat{\vec{p}}=\cdots
\end{equation}

\begin{align}
    [\hat{L}_1,\hat{L}_2]&=[x_2p_3-x_3p_2,x_3p_1-x_1p_3]\\
    [A+B,C+D]&=[A+B,C]+[A+B,D]\\
    &=[A,C]+[B,C]+[A,D]+[B,D]\\
    \Rightarrow
    [L_1,L_2]&=\underset{\mbox{I}}{[x_2p_3,x_3p_1]}-\underset{\mbox{II}}{[x_3p_2,x_3p_1]}-\underset{\mbox{III}}{[x_2p_3,x_1p_3]}+\underset{\mbox{IV}}{[x_3p_2,x_1p_3]}
\end{align}

\begin{align}
    [A,BC]&=B[A,C]+[A,B]C \\
    [AB,C]&=A[B,C]+[A,C]B
\end{align}

\begin{align}
    [x_i,p_j]=i\hbar\delta_{ij},\ [p_i,x_j]=-i\hbar\delta_{ij}
\end{align}

\begin{align}
    [x_i,x_j]=[p_i,p_j]=0
\end{align}

\begin{align}
    \mbox{I}
    &=[x_2p_3,x_3]p_1+x_3[x_2p_2,p_1]\\
    &=[x_2,x_3]p_3p_1+x_2[p_3,x_3]p_1+x_3[x_2,p_1]p_3+x_2x_3[p_3,p_1]\\
    &=-i\hbar x_2p_1\\
    \mbox{II}
    &=[x_3p_2,x_3]p_1+x_3[x_3p_2,p_1]\\
    &=x_3[p_2,x_3]p_1++[x_3,x_3]p_1p_2+x_3x_3[p_2,p_1]+x_3[x_3,p_1]p_2\\
    &=0\\
    \mbox{III}
    &=[x_2p_3,x_1]p_3+x_1[x_2p_3,p_3]=0\\
    \mbox{IV}
    &=[x_3p_2,x_1]p_3+x_1[x_3p_2,p_3]\\
    &=[x_3,x_1]p_2p_3+x_3[p_2,x_1]p_3+x_1[x_3,p_3]p_2+x_1x_3[p_2,p_3]\\
    &=i\hbar x_1p_2
\end{align}

\begin{align}
    [L_1,L_2]&=i\hbar(x_1p_2-x_2p_1)=i\hbar L_3
\end{align}

\begin{align}
    [L_i,L_j]=\varepsilon_{ijk}i\hbar L_k
\end{align}

\item[(b)]

\begin{align}
    [\hat{\vec{L}}_1^2,\hat{L}_1]
\end{align}

\begin{align}
    \hat{\vec{L}}^2&=\hat{L}_1^2+\hat{L}_2^2+\hat{L}_3^2\\
    &=[L_1^2+L_2^2+L_3^2,L_1]=0\\
    &=[L_2^2,L_1]+[L_3^2,L_1]\\
    &=L_2[L_2,L_1]+[L_2,L_1]L_2+L_3[L_3,L_1]+[L_3,L_1]L_3\\
        &=-i\hbar L_2L_3-i\hbar L_3L_2+i\hbar L_3L_2+i\hbar L_2L_3\\
&=-i\hbar(L_2L_3+L_3L_2)+i\hbar(L_3L_2+L_2L_3)=0
\end{align}

\item[(c)]

\begin{align}
    \vec{L}\times\vec{L}&=
    \begin{bmatrix}
    x_2p_3-x_3p_2 \\
    x_3p_1-x_1p_3 \\
    x_1p_2-x_2p_1
    \end{bmatrix}
    \times
    \begin{bmatrix}
x_2p_3-x_3p_2 \\
x_3p_1-x_1p_3 \\
x_1p_2-x_2p_1
    \end{bmatrix}\\&=
    \begin{bmatrix}
    (x_3p_1-x_1p_3)(x_1p_2-x_2p_1)-(x_1p_2-x_2p_1)(x_3p_1-x_1p_3)\\
    (x_1p_2-x_2p_1)(x_2p_3-x_3p_2)-(x_2p_3-x_3p_2)(x_1p_2-x_2p_1)\\
    (x_2p_3-x_3p_2)(x_3p_1-x_1p_3)-(x_3p_1-x_1p_3)(x_2p_3-x_3p_2)
    \end{bmatrix}\\&=
    \begin{bmatrix}
    [L_2,L_3] \\
    [L_3,L_1] \\
    [L_1,L_2]
    \end{bmatrix}=0
\end{align}

\begin{align}
    (\vec{L}\times\vec{L})_l=\sum_{m,n}\varepsilon_{lmn}L_mL_n=\varepsilon_{lmn}(L_mL_n-L_nL_m)=\varepsilon_{lmn}[L_m,L_n]=i\hbar L_l
\end{align}

\item[(d)]

\begin{align}
    [\frac{p^2}{2m},x_i]&=\frac{1}{2m}[p^2,x_i]\\
    &=\frac{1}{2m}[p_1^2+p_2^2+p_3^2,x_i]\\
    &=\frac{1}{2m}[p_i^2,x_i]\\
    &=\frac{1}{2m}(p_i[p_i,x_i]+[p_i,x_i]p_i)\\
    &=\frac{1}{2m}(p_i(-i\hbar)-i\hbar p_i)\\
    &=\frac{-i\hbar}{m}p_i
\end{align}

\begin{align}
    [V(x),p_i]\psi
    &=(V(-i\hbar\partial_{x_i})-(-i\hbar\partial_{x_i})V)\psi\\
    &=V(-i\hbar)\partial_{x_i}\psi-(-i\hbar)\partial_{x_i}(V\psi)\\
    &=V(-i\hbar)\partial_{x_i}\psi-V(-i\hbar)\partial_{x_i}\psi-(-i\hbar)(\partial_{x_i}V)\psi\\
    &=\underset{[V(x),p_i]}{\underbrace{i\hbar(\partial_{x_i}V)}}\psi
\end{align}

\begin{align}
    [L_1,x_1]=[x_2p_3-x_3p_2,x_1]=0
\end{align}

\begin{align}
    [L_1,x_2]
    &=[x_2p_3-x_3p_2,x_2]\\
    &=[x_2p_3,x_2]-[x_3p_2,x_2]\\
    &=x_2[p_3,x_2]+[x_2,x_2]p_3-(x_3[p_2,x_2]+[x_3,x_2]p_2)\\
    &=-x_3[p_2,x_2]\\
    &=i\hbar x_3
\end{align}

\end{enumerate}

\newpage

\paragraph{Question 4}

\begin{enumerate}
\item[(a)]

\begin{align}
    \psi(x,0)=Ae^{ik_0x}e^{\frac{-x^2}{2b^2}}
\end{align}

\begin{align}
    \rho(x,0)=|\psi(x,0)|^2=\psi^*\psi
\end{align}
is the probability density of the wave function

\begin{align}
    \rho(x,0)dx
\end{align}
is the probability to find the particle in $(x,x+dx)$

therefore,
    \begin{align}
    1&=\int_{-\infty}^\infty\rho(x,0)dx\\
    &=A^2\int e^{-\frac{x^2}{b^2}}dx\\
    (u=\frac{x}{b})&=A^2b\int e^{-u^2}du\\
    &=A^2b\sqrt{\pi}\\
    \Rightarrow A&=\frac{1}{\sqrt{b}\sqrt[4]{\pi}}
\end{align}

\item[(b)]

\begin{align}
    \tilde{\psi}(k)&=\int^\infty_{-\infty} dx e^{-ikx}\psi(x,0)
\end{align}

\begin{align}
    \tilde{\psi}(k)
    &=\frac{1}{\sqrt{b}\sqrt[4]{\pi}}\int^\infty_{-\infty} dx e^{-ikx}e^{ik_0x}e^{\frac{-x^2}{2b^2}}\\
    &=\frac{1}{\sqrt{b}\sqrt[4]{\pi}}\int^\infty_{-\infty} dx \exp{\bigg[-i(k-k_0)x-\frac{x^2}{2b^2}\bigg]}\\
    &=\frac{1}{\sqrt{b}\sqrt[4]{\pi}}\int^\infty_{-\infty} dx \exp{\bigg[-\frac{1}{2b^2}\Big(x^2+2b^2i(k-k_0)x-b^4(k-k_0)^2\Big)-\frac{b^2}{2}(k-k_0)^2\bigg]}\\
    &=\frac{1}{\sqrt{b}\sqrt[4]{\pi}}\int^\infty_{-\infty} dx \exp{\bigg[-\frac{1}{2b^2}\Big(x+b^2i(k-k_0)\Big)^2-\frac{b^2}{2}(k-k_0)^2\bigg]}\\
    &=\frac{1}{\sqrt{b}\sqrt[4]{\pi}}e^{-\frac{b^2}{2}(k-k_0)^2}\int^\infty_{-\infty} dx \exp{\bigg[-\frac{1}{2b^2}\Big(x+b^2i(k-k_0)\Big)^2\bigg]}\\
    &=\frac{1}{\sqrt{b}\sqrt[4]{\pi}}e^{-\frac{b^2}{2}(k-k_0)^2}\int^\infty_{-\infty} dx' \exp{\bigg[-\frac{x'^2}{2b^2}\bigg]}\\
    &=\frac{1}{\sqrt{b}\sqrt[4]{\pi}}e^{-\frac{b^2}{2}(k-k_0)^2}\sqrt{2b}\int^\infty_{-\infty} dx'' \exp{[-x''^2]}\\
    &=\frac{1}{\sqrt{b}\sqrt[4]{\pi}}e^{-\frac{b^2}{2}(k-k_0)^2}\sqrt{2b\pi}\\
    &=\sqrt{2b\sqrt{\pi}}e^{-\frac{b^2}{2}(k-k_0)^2}
\end{align}

\item[(c)]

\begin{align}
    (\tilde{\psi}(k))^2&=e^{-b^2(k-k_0)^2}2b\sqrt{\pi}\\
    \Rightarrow e^{-1}&=e^{-b^2(k-k_0)^2}\\
    -1&=-b^2(k-k_0)^2\\
    \frac{1}{b}&=|k-k_0|=\frac{1}{2}\Delta k
\end{align}
\item[(d)]

\begin{align}
    \psi(x,t)
    &=\int^\infty_{-\infty} \frac{dk}{2\pi}\exp{\bigg[i\Big(kx-\frac{\hbar k^2}{2m}t\Big)\bigg]}\tilde{\psi}(k)\\
    &=\int^\infty_{-\infty} \frac{dk}{2\pi}\exp{\bigg[i\Big(kx-\frac{\hbar k^2}{2m}t\Big)\bigg]}\sqrt{2b\sqrt{\pi}}e^{-\frac{b^2}{2}(k-k_0)^2}\\
    &=\frac{\sqrt{2b\sqrt{\pi}}}{2\pi}\int^\infty_{-\infty} dk\exp{\bigg[i\Big(kx-\frac{\hbar k^2}{2m}t\Big)-\frac{b^2}{2}(k-k_0)^2\bigg]}\\
    &=\frac{\sqrt{2b\sqrt{\pi}}}{2\pi}\int^\infty_{-\infty} dk\exp{\bigg[ikx-\frac{\hbar k^2}{2m}it-\frac{b^2}{2}k^2+b^2kk_0-\frac{b^2}{2}k_0^2\bigg]}\\
    &=\frac{\sqrt{2b\sqrt{\pi}}}{2\pi}e^{-\frac{b^2}{2}k_0^2}\int^\infty_{-\infty} dk\exp{\bigg[ikx-\frac{\hbar k^2}{2m}it-\frac{b^2}{2}k^2+b^2kk_0\bigg]}\\
    &=\frac{\sqrt{2b\sqrt{\pi}}}{2\pi}e^{-\frac{b^2}{2}k_0^2}\int^\infty_{-\infty} dk\exp{\bigg[k(ix+b^2k_0)+k^2\Big(-\frac{\hbar}{2m}it-\frac{b^2}{2}\Big)\bigg]}\\
    &=\frac{\sqrt{2b\sqrt{\pi}\pi}}{2\pi}e^{-\frac{b^2}{2}k_0^2}\frac{1}{\sqrt{\frac{\hbar}{2m}it+\frac{b^2}{2}}}\exp{\bigg[\frac{(ix+b^2k_0)^2}{4(\frac{\hbar}{2m}it+\frac{b^2}{2})}\bigg]}\\
    &=\frac{\sqrt{b}}{\sqrt{\pi}\sqrt{\frac{\hbar}{m}it+b^2}}\exp{\bigg[\frac{(ix+b^2k_0)^2}{2(\frac{\hbar}{m}it+b^2)}-\frac{b^2}{2}k_0^2\bigg]}
\end{align}

\item[(e)]

\end{enumerate}
\end{document}